Start specifying some abstraction of log layout

src/Examples/Logging/HoareProof.v
@@ -3,8 +3,7 @@ Require Import POCS.
 Require Import Examples.Logging.Impl.
 Require Import Helpers.Array.
 
-Module D := OneDisk.
-Module TxnD := TxnDisk.
+Require Import Spec.HoareTactics.
 
 Record LogicalState :=
   { ls_disk : disk;
@@ -29,6 +28,49 @@ Inductive LogDecode (d: disk) (ls: LogicalState) : Prop :=
                        sel desc.(addresses) i = a /\
                        diskGet d (2 + i) = Some b):
     LogDecode d ls.
+
+Definition disk_invariant (d: disk) :=
+  diskSize d >= 2 + LOG_LENGTH.
+
+Record PhysicalState :=
+  { p_hdr: LogHdr;
+    p_desc: Descriptor;
+    p_log_values: list block;
+    p_data_region: disk; }.
+
+Definition PhyDecode (d: disk) : option PhysicalState :=
+  match diskGet d 0, diskGet d 1 with
+  | Some bhdr, Some bdesc =>
+    Some {| p_hdr := LogHdr_fmt.(decode) bhdr;
+            p_desc := Descriptor_fmt.(decode) bdesc;
+            p_log_values := diskSubslice d 2 (LOG_LENGTH);
+            p_data_region := diskSubslice d (2+LOG_LENGTH) (diskSize d - (2 + LOG_LENGTH)); |}
+  | _, _ => None
+  end.
+
+Theorem PhyDecode_invariant : forall d,
+    disk_invariant d ->
+    exists ps, PhyDecode d = Some ps /\
+          (exists b, diskGet d 0 = Some b /\
+                LogHdr_fmt.(decode) b = ps.(p_hdr)) /\
+          (exists b, diskGet d 1 = Some b /\
+                Descriptor_fmt.(decode) b = ps.(p_desc)) /\
+          length ps.(p_log_values) = LOG_LENGTH /\
+          2 + LOG_LENGTH + diskSize ps.(p_data_region) = diskSize d.
+Proof.
+  unfold disk_invariant; intros.
+  unfold PhyDecode.
+  edestruct (@disk_inbounds_exists 0 d); try omega.
+  edestruct (@disk_inbounds_exists 1 d); try omega.
+  repeat simpl_match.
+  descend; (intuition idtac);
+    cbn [p_hdr p_desc p_log_values p_data_region].
+  - descend; intuition eauto.
+  - descend; intuition eauto.
+  - simpl; autorewrite with disk_size; auto.
+  - autorewrite with disk_size.
+    omega.
+Qed.
 
 Inductive CommitStatus d b : Prop :=
 | commit_status bhdr 
@@ -94,3 +136,145 @@ Definition log_recover_spec ls : Specification block unit D.State :=
                        CommitStatus state' false;
       alternate := fun state' _ => state = state'
     |}.
+
+Ltac simplify :=
+  repeat match goal with
+         | _ => progress propositional
+         end.
+
+Ltac finish :=
+  repeat match goal with
+         | _ => auto
+         | _ => congruence
+         end.
+
+(* specs for one-disk primitives (restatement of semantics as specs) *)
+Ltac prim :=
+  eapply proc_cspec_impl; [ unfold spec_impl | eapply op_spec_sound ];
+    simpl;
+    propositional;
+    (intuition auto);
+    propositional.
+
+Theorem read_ok a :
+  proc_cspec D.ODLayer
+             (read a)
+             (fun state =>
+                {| pre := True;
+                   post state' r :=
+                     diskGet state a ?|= eq r /\
+                     state' = state;
+                   alternate state' _ :=
+                     state' = state; |}).
+Proof.
+  unfold read.
+  prim;
+    repeat match goal with
+           | [ H: D.op_step _ _ _ _ |- _ ] => invert H; clear H
+           end;
+    propositional;
+    auto.
+  destruct (diskGet s' a); simpl; eauto.
+Qed.
+
+Theorem write_ok a v :
+  proc_cspec D.ODLayer
+             (write a v)
+             (fun state =>
+                {| pre := True;
+                   post state' r :=
+                     r = tt /\
+                     state' = diskUpd state a v;
+                   alternate state' _ :=
+                     state' = state \/
+                     state' = diskUpd state a v; |}).
+Proof.
+  unfold write.
+  prim;
+    repeat match goal with
+           | [ H: D.op_step _ _ _ _ |- _ ] => invert H; clear H
+           end;
+    propositional;
+    auto.
+Qed.
+
+Theorem size_ok :
+  proc_cspec D.ODLayer
+             (size)
+             (fun state =>
+                {| pre := True;
+                   post state' r :=
+                     r = diskSize state /\
+                     state' = state;
+                   alternate state' _ :=
+                     state' = state; |}).
+Proof.
+  unfold size.
+  prim;
+    repeat match goal with
+           | [ H: D.op_step _ _ _ _ |- _ ] => invert H; clear H
+           end;
+    propositional;
+    auto.
+Qed.
+
+Hint Resolve read_ok write_ok size_ok.
+
+Ltac step :=
+  unshelve step_proc; simplify; finish.
+
+Opaque diskGet.
+
+Theorem gethdr ps :
+  proc_cspec D.ODLayer
+             gethdr
+             (fun state =>
+                {| pre := disk_invariant state /\
+                          PhyDecode state = Some ps;
+                   post state' r :=
+                     r = ps.(p_hdr) /\
+                     state' = state;
+                   alternate state' _ :=
+                     state' = state; |}).
+Proof.
+  unfold gethdr.
+  step.
+  step.
+  eapply PhyDecode_invariant in H; propositional; eauto.
+  replace (diskGet state 0) in *; simpl in *; propositional; eauto.
+  congruence.
+Qed.
+
+Theorem writedesc ps desc :
+  proc_cspec D.ODLayer
+             (writedesc desc)
+             (fun state =>
+                {| pre := disk_invariant state /\
+                          PhyDecode state = Some ps;
+                   post state' r :=
+                     disk_invariant state' /\
+                     exists ps', PhyDecode state' = Some ps' /\
+                            ps' = {| p_hdr := ps.(p_hdr);
+                                     p_desc := desc;
+                                     p_log_values := ps.(p_log_values);
+                                     p_data_region := ps.(p_data_region); |};
+                   alternate state' _ :=
+                     disk_invariant state' /\
+                     exists ps', PhyDecode state' = Some ps' /\
+                            ps' = ps \/
+                            ps' = {| p_hdr := ps.(p_hdr);
+                                     p_desc := desc;
+                                     p_log_values := ps.(p_log_values);
+                                     p_data_region := ps.(p_data_region); |};
+                   |}).
+Proof.
+  unfold writedesc.
+  eapply proc_cspec_impl; [ unfold spec_impl | solve [eauto] ];
+    simpl;
+    propositional;
+    (intuition auto);
+    propositional.
+  - unfold disk_invariant in *.
+    autorewrite with upd; auto.
+  - eexists; intuition eauto.
+Abort.
